WIP

FO-proof-systems/Sema.thy
@@ -13,8 +13,8 @@ term "None"
 
 locale formula_semantics = formula_syntax subst
   for subst::"'v \<Rightarrow> 'c \<Rightarrow> 'p \<Rightarrow> 'p"
-+
-fixes dom::"'t \<Rightarrow> 'c list"
+  +
+  fixes dom::"'t \<Rightarrow> 'c list"
 begin
 
 find_theorems name: "list*find"
@@ -48,7 +48,7 @@ termination formula_semantics
 abbreviation valid ("\<Turnstile> _" 51) where
 "\<Turnstile> F \<equiv> \<forall>A. A \<Turnstile> F"
 
-definition entailment :: "('p, 'v, 't) formula set \<Rightarrow> ('p, 'v, 't) formula \<Rightarrow> bool" 
+definition formula_entailment :: "('p, 'v, 't) formula set \<Rightarrow> ('p, 'v, 't) formula \<Rightarrow> bool" 
   (infix "\<TTurnstile>" 63) where
 "\<Gamma> \<TTurnstile> F \<equiv> (\<forall>\<A>. ((\<forall>G \<in> \<Gamma>. \<A> \<Turnstile> G) \<longrightarrow> (\<A> \<Turnstile> F)))"
 
